gf128 wip

examples/low-level/crypto/Crypto.Symmetric.GF128.Spec.fst
@@ -1,17 +1,67 @@
 module Crypto.Symmetric.GF128.Spec
 
-open Crypto.Symmetric.Bytes 
-
-module U128 = FStar.UInt128
+open Crypto.Symmetric.Bytes
+open FStar.Int.Cast
+open FStar.UInt128
+open FStar.UInt
 
 type text = Seq.seq (lbytes 16)
-type elem = U128.t
+type elem = FStar.UInt128.t
 
 val op_Plus_At: elem -> elem -> Tot elem
-let op_Plus_At x y = U128.(x ^^ y)
+let op_Plus_At x y = x ^^ y
 
-val op_Star_At: elem -> elem -> Tot elem
-let op_Star_At x y = U128.(x ^^ y) // FAKE IMPLEMENTATION TODO FIX
+let ones_128 = uint_to_t (ones 128)
+let zero_128 = uint_to_t (zero 128)
+
+val ith_bit_mask: num:elem -> i:nat{i < 128} -> Pure elem
+  (requires True)
+  (ensures (fun r ->
+    nth (v num) i = true ==> r = ones_128 /\
+    nth (v num) i = false ==> r = zero_128))
+let ith_bit_mask num i = if (nth (v num) i) then ones_128 else zero_128
+
+val shift_right: elem -> Tot elem
+let shift_right a = a >>^ 1ul
+
+private let r_mul = uint64_to_uint128(225uL) <<^ 120ul
+
+val mask_add: a:elem -> b:elem -> r:elem -> dep:nat{dep < 128} -> Pure elem
+  (requires True)
+  (ensures (fun s -> 
+    nth (v b) dep = true ==> s = r +@ a /\
+    nth (v b) dep = false ==> s = r))
+  (decreases (128 - dep))
+let mask_add a b r dep =
+  let msk = ith_bit_mask b dep in
+  let m = a &^ msk in
+  r +@ m
+
+val shift_right_modulo: a:elem -> Pure elem
+  (requires True)
+  (ensures (fun r ->
+    nth (v a) 127 = true ==> r = (shift_right a) +@ r_mul /\
+    nth (v a) 127 = false ==> r = shift_right a))
+let shift_right_modulo a =
+  let msk = ith_bit_mask a 127 in
+  let m = r_mul &^ msk in
+  shift_right a +@ m
+
+#set-options "--z3rlimit 15 --max_fuel 1 --initial_fuel 1"
+
+val mul_loop: a:elem -> b:elem -> r:elem -> dep:nat{dep <= 128} -> Tot elem
+  (decreases (128 - dep))
+let rec mul_loop a b r dep =
+  if dep = 128 then r else
+  begin
+    let nr = mask_add a b r dep in 
+    let na = shift_right_modulo a in
+    mul_loop na b nr (dep + 1)
+  end
+
+val op_Star_At: a:elem -> b:elem -> Tot elem
+let op_Star_At a b = mul_loop a b zero_128 0
+
 
 assume val add_comm: a:elem -> b:elem -> Lemma (a +@ b == b +@ a)
 
@@ -22,22 +72,6 @@ val encode:lbytes 16 -> Tot elem
 let encode b = zero // FAKE IMPLEMENTATION TODO FIX
 val decode:elem -> Tot (lbytes 16)
 let decode e = Seq.create 16 0uy
-
-
-
-(*
-val add_loop: l:nat -> lbytes l -> lbytes l -> Tot (lbytes l)
-
-
-val add_loop: l:nat{ l <= 16 } -> lbytes l -> lbytes l -> Tot (lbytes l)
-let rec add_loop l a b = 
-  if l = 0 then Seq.createEmpty 
-  else
-    let r = add_loop (l-1) (tail a) (tail b) in 
-    cons (UInt8.logxor (head a) (head b)) r
-
-let op_Plus_At a b = add_loop 16 a b
-*)
 
 open FStar.Seq
 open FStar.SeqProperties 
